lib/steel/Steel.Effect.Common.fsti
@@ -155,7 +155,7 @@ noextract
 let hmem (p:vprop) = hmem (hp_of p)
 
 /// Abstract predicate for vprop implication. Currently implemented as an implication on the underlying slprop
-val can_be_split (p q:pre_t) : Type0
+val can_be_split (p q:pre_t) : prop
 
 /// Exposing the implementation of `can_be_split` when needed for proof purposes
 val reveal_can_be_split (_:unit) : Lemma
@@ -252,7 +252,7 @@ let can_be_split_forall_dep_congr_r
 
 /// To simplify the implementation of the framing tactic, dependent equivalence
 /// is defined as a double dependent implication
-let equiv_forall (#a:Type) (t1 t2:post_t a) : Type0
+let equiv_forall (#a:Type) (t1 t2:post_t a) : prop
   = t1 `can_be_split_forall` t2 /\ t2 `can_be_split_forall` t1
 
 /// This equivalence models a context restriction at the end of a Steel computation;
@@ -308,9 +308,9 @@ val reveal_mk_rmem (r:vprop) (h:hmem r) (r0:vprop{r `can_be_split` r0})
 
 (* Logical pre and postconditions can only access the restricted view of the heap *)
 
-type req_t (pre:pre_t) = rmem pre -> Type0
+type req_t (pre:pre_t) = rmem pre -> prop
 type ens_t (pre:pre_t) (a:Type) (post:post_t a) =
-  rmem pre -> (x:a) -> rmem (post x) -> Type0
+  rmem pre -> (x:a) -> rmem (post x) -> prop
 
 (* Empty assertion *)
 val emp : vprop
@@ -369,7 +369,7 @@ open FStar.Tactics.V2
 [@@ __steel_reduce__; strict_on_arguments [0]]
 let rec frame_equalities'
   (frame:vprop)
-  (h0:rmem frame) (h1:rmem frame) : Type0
+  (h0:rmem frame) (h1:rmem frame) : prop
   = begin match frame with
     | VUnit p -> h0 frame == h1 frame
     | VStar p1 p2 ->
@@ -391,18 +391,18 @@ let rec frame_equalities'
 /// The uncommon formulation with an extra [p] is needed to use in `rewrite_with_tactic`,
 /// where the goal is of the shape `frame_equalities frame h0 h1 == ?u`
 /// The rewriting happens below, in `frame_vc_norm`
-val lemma_frame_equalities (frame:vprop) (h0:rmem frame) (h1:rmem frame) (p:Type0)
+val lemma_frame_equalities (frame:vprop) (h0:rmem frame) (h1:rmem frame) (p:prop)
   : Lemma
     (requires (h0 frame == h1 frame) == p)
     (ensures frame_equalities' frame h0 h1 == p)
 
 /// A special case for frames about emp.
-val lemma_frame_emp (h0:rmem emp) (h1:rmem emp) (p:Type0)
+val lemma_frame_emp (h0:rmem emp) (h1:rmem emp) (p:prop)
   : Lemma (requires True == p)
           (ensures frame_equalities' emp h0 h1 == p)
 
 /// A variant of conjunction elimination, suitable to the equality goals during rewriting
-val elim_conjunction (p1 p1' p2 p2':Type0)
+val elim_conjunction (p1 p1' p2 p2':prop)
   : Lemma (requires p1 == p1' /\ p2 == p2')
           (ensures (p1 /\ p2) == (p1' /\ p2'))
 
@@ -1694,7 +1694,7 @@ let normal_tac_steps = [primops; iota; zeta; delta_only [
 let normal_tac (#a:Type) (x:a) : a = FStar.Pervasives.norm normal_tac_steps x
 
 /// Helper lemma to establish relation between normalized and initial values
-let normal_elim (x:Type0) : Lemma
+let normal_elim (x:prop) : Lemma
   (requires x)
   (ensures normal_tac x)
   = ()
@@ -1742,18 +1742,18 @@ let close_equality_typ (t:term) : Tac unit =
 /// The following three lemmas are helpers to manipulate the goal in canon_l_r
 
 [@@ no_subtyping]
-let inst_bv (#a:Type) (#p:a -> Type0) (#q:Type0) (x:a) (_:squash (p x ==> q))
+let inst_bv (#a:Type) (#p:a -> prop) (#q:prop) (x:a) (_:squash (p x ==> q))
   : Lemma ((forall (x:a). p x) ==> q) = ()
 
-let modus_ponens (#p #q:Type0) (_:squash p)
+let modus_ponens (#p #q:prop) (_:squash p)
   : Lemma ((p ==> q) ==> q)
   = ()
 
-let cut (p q:Type0) : Lemma (requires p /\ (p ==> q)) (ensures q) = ()
+let cut (p q:prop) : Lemma (requires p /\ (p ==> q)) (ensures q) = ()
 
-let and_true (p: Type0) : Lemma (requires (p /\ (p ==> True))) (ensures p) = ()
+let and_true (p: prop) : Lemma (requires (p /\ (p ==> True))) (ensures p) = ()
 
-let solve_implies_true (p: Type0) : Lemma (p ==> True) = ()
+let solve_implies_true (p: prop) : Lemma (p ==> True) = ()
 
 // This exception is raised for failures that should not be considered
 // hard but should allow postponing the goal instead
@@ -1770,7 +1770,7 @@ let is_and (t:term) : bool =
 
 private
 let is_squash (t:term) : bool =
-  is_any_fvar t [`%squash; `%auto_squash]
+  is_any_fvar t [`%squash]
 
 private
 let is_star (t:term) : bool =
@@ -1804,22 +1804,17 @@ let rec unify_pr_with_true (pr: term) : Tac unit =
         // postpone the goal instead of failing hard, to allow for other goals to solve those uvars
         raise (Postpone "unify_pr_with_true: some uvars are still there")
 
-let elim_and_l_squash (#a #b: Type0) (#goal: Type0) (f: (a -> Tot (squash goal))) (h: (a /\ b)) : Tot (squash goal) =
-  let f' (x: squash a) : Tot (squash goal) =
-    FStar.Squash.bind_squash x f
-  in
-  let elim_impl (x: squash (a /\ b)) : Tot (squash a) = () in
-  f' (elim_impl (FStar.Squash.return_squash h))
+let elim_and_l_squash (#a #b: prop) (#goal: prop) (f: a -> Tot (squash goal)) (h: (a /\ b)) : Tot (squash goal) =
+  f ()
 
-let elim_and_r_squash (#a #b: Type0) (#goal: Type0) (f: (b -> Tot (squash goal))) (h: (a /\ b)) : Tot (squash goal) =
-  let f' (x: squash b) : Tot (squash goal) =
-    FStar.Squash.bind_squash x f
-  in
-  let elim_impl (x: squash (a /\ b)) : Tot (squash b) = () in
-  f' (elim_impl (FStar.Squash.return_squash h))
+let elim_and_r_squash (#a #b: prop) (#goal: prop) (f: b -> Tot (squash goal)) (h: (a /\ b)) : Tot (squash goal) =
+  f ()
 
-let _return_squash (#a: Type) () (x: a) : Tot (squash a) =
-  FStar.Squash.return_squash x
+let _return_squash (#a: prop) () (x: a) : Tot (squash a) =
+  ()
+
+let elim_squash (#inner #goal: prop) (f: inner -> Tot (squash goal)) (h: squash inner) : Tot (squash goal) =
+  f ()
 
 let rec set_abduction_variable_term (pr: term) : Tac term =
   let hd, tl = collect_app pr in
@@ -1848,9 +1843,19 @@ let rec set_abduction_variable_term (pr: term) : Tac term =
 let set_abduction_variable () : Tac unit =
   let g = cur_goal () in
   match inspect_unascribe g with
-  | Tv_Arrow b _ ->
+  | Tv_Arrow b _ -> (
     let pr = b.sort in
-    exact (set_abduction_variable_term pr)
+    // In the prop world, the precondition is wrapped in a `squash`.
+    // Peel it off, set the abduction variable on the underlying prop,
+    // and re-wrap with `elim_squash`.
+    let hd, tl = collect_app pr in
+    match unsquash_term pr with
+    | Some inner ->
+      let arg = set_abduction_variable_term inner in
+      exact (mk_app (`elim_squash) [arg, Q_Explicit])
+    | _ ->
+      exact (set_abduction_variable_term pr)
+  )
   | _ -> fail "Not an arrow goal"
 
 let canon_l_r (use_smt:bool)
@@ -2028,7 +2033,7 @@ let canon_l_r (use_smt:bool)
       //G3 is the lhs of the implication in the auxiliary goal
       //  that we have in our assumptions via b
 
-      apply (`FStar.Squash.return_squash);
+      // apply (`FStar.Squash.return_squash);
       exact (binding_to_term b)
     end);
 
@@ -3121,15 +3126,9 @@ let init_resolve_tac' (dict: _) : Tac unit =
 [@@ resolve_implicits; framing_implicit; plugin]
 let init_resolve_tac () : Tac unit = init_resolve_tac' []
 
-(* AF: There probably is a simpler way to get from p to squash p in a tactic, so that we can use apply_lemma *)
-let squash_and p (x:squash (p /\ True)) : (p /\ True) =
-  let x : squash (p `Prims.pair` True) = FStar.Squash.join_squash x in
-  x
-
 /// Calling into the framing tactic to ensure that the vprop whose selector we are trying to access is in the context
 [@@plugin]
 let selector_tactic () : Tac unit =
-  apply (`squash_and);
   apply_lemma (`intro_can_be_split_frame);
   flip ();
   norm [delta_only [
