lib/steel/Steel.ST.GenElim.fsti
@@ -22,7 +22,7 @@ val gen_elim
   (#[@@@ defer_to framing_implicit] post: Ghost.erased a -> Tot prop)
   (#[@@@ defer_to framing_implicit] sq: squash (gen_elim_prop_placeholder true p a q post))
   (_: unit)
-: STGhostF (Ghost.erased a) opened p (fun x -> guard_vprop (q x)) ( (T.with_tactic solve_gen_elim_prop) (squash (gen_elim_prop true p a q post))) post
+: STGhostF (Ghost.erased a) opened p (fun x -> guard_vprop (q x)) ( (T.with_tactic solve_gen_elim_prop) (gen_elim_prop true p a q post)) post
 
 val gen_elim_dep
   (#opened: _)
@@ -32,4 +32,4 @@ val gen_elim_dep
   (#[@@@ defer_to framing_implicit] post: Ghost.erased a -> Tot prop)
   (#[@@@ defer_to framing_implicit] sq: squash (gen_elim_prop_placeholder false p a q post))
   (_: unit)
-: STGhostF (Ghost.erased a) opened p (fun x -> guard_vprop (q x)) ( (T.with_tactic solve_gen_elim_prop) (squash (gen_elim_prop false p a q post))) post
+: STGhostF (Ghost.erased a) opened p (fun x -> guard_vprop (q x)) ( (T.with_tactic solve_gen_elim_prop) (gen_elim_prop false p a q post)) post
